This is a TV that checks the semantics preservation (but not correctnes) of Softbound.   1) redefined TV by Fixpoint, and proved its properties by Lemma.      the old version of TV is defined by Lemma directly, which is not      quite convenient when proving its property.   2) checked if the output program's memory effects are a super set of      its input's, because Softbound introduces additonal      alloca/load/store.
     The current design is ad-hoc, and obviously unsafe, which simply
     checks is the output smem includes the input's. It should be fine
     for alloca and load, but assuming that the additional stores are at a
     disjoint space like in Softbound.

     The problem is that LLVM's memory state is not SSA, so we only have
     only symbol to represent the mem-state. This is different from
     non-memory variabls that are SSA, so it is easy to reason about
     their effects. A possible solution is extending LLVM mem-state to
     be a SSA form, namely disjoint memory regions have different mem
     symbol. This should be useful for Softbound proofs, since we at
     least need to prove that users' mem-space and metadata-space are 
     disjoint. Plus, proving alias analysis might also need this idea to 
     reason about 'Point-to' relations.
  3) Makefile in vol/src/Parser/tvcases runs some simple cases --- Input.ll 
     and Output.ll, and in/out programs of Softbound (vol/tests/*)

     The TV works for most of them, except two cases of Softbound --- 
     globals and funcret. Because
       a) Softbound changes temporary variale names (%1, %2, ...) for
          globals, and callsite of a function that returns a pointer,
          while the TV assumes the tmp names are kept and unchanged.

          Handling tmp vars renaming may not be what we are interested
          in, and can be solved if Softbound can tell us the mapping...
       b) %v = func (..) is translated to
          call func (%p,...); %v = load %p
          if func returns a pointer. The TV does not consider this case.
       c) Softbound can change tail-call functions to non-tail-call, say
          atoi in the input is a tail-call, but its output counter-part
          softbound_atoi that has a wrapper is of non-tail-call. Our
          opsem does not distinguish if it is tail-call. So it does not
          matter so far.



git-svn-id: https://webdav.seas.upenn.edu/svn/sol/vol@2815 eef5ea85-cc2e-0410-bd84-0fae1f012da8

src/myocamlbuild.ml
@@ -19,4 +19,4 @@ ocaml_lib ~extern:true "eq_tv";;
 ocaml_lib ~extern:true "sub_tv";;
 
 flag ["link"; "ocaml"; "g++"] (S[A"-cc"; A"g++"]);;
-dep ["link"; "ocaml"; "use_bindings"] ;;
+dep ["link"; "ocaml"; "use_bindings"; "using_sub_tv"; "using_eq_tv"] ;;
