src/TV/sub_tv.v
@@ -17,8 +17,7 @@ Require Import opsem_pp.
 Require Import trace.
 Require Import symexe_def.
 Require Import symexe_lib.
-Require Import symexe_complete.
-Require Import symexe_sound.
+Require Import symexe_tactic.
 Require Import seop_llvmop.
 Require Import assoclist.
 Require Import ssa_props.
@@ -27,6 +26,159 @@ Require Import sub_tv_dec.
 Require Import Coq.Bool.Sumbool.
 
 Export SimpleSE.
+
+(* This is the tricky part. How can we know sm2 includes sm1 ?
+ * So far, we only consider the memory effects of Softbound. 
+ *
+ * The axiom assumes the memory behavior of a lib call. This should
+ * be admissible in terms of other axioms.
+*)
+Axiom smem_lib_sub : id -> bool.
+
+Definition tv_value (v v':value) := sumbool2bool _ _ (value_dec v v').
+Definition tv_typ (t t':typ) := sumbool2bool _ _ (typ_dec t t').
+Definition tv_align (a a':align) := sumbool2bool _ _ (Align.dec a a').
+
+Fixpoint tv_sterm (st st':sterm) : bool :=
+match (st, st') with
+| (sterm_val v, sterm_val v') => tv_value v v'
+| (sterm_bop b sz st1 st2, sterm_bop b' sz' st1' st2') =>
+  sumbool2bool _ _ (bop_dec b b') && sumbool2bool _ _ (Size.dec sz sz') &&
+  tv_sterm st1 st1' && tv_sterm st2 st2'
+| (sterm_fbop b f st1 st2, sterm_fbop b' f' st1' st2') =>
+  sumbool2bool _ _ (fbop_dec b b') && 
+  sumbool2bool _ _ (floating_point_dec f f') &&
+  tv_sterm st1 st1' && tv_sterm st2 st2'
+| (sterm_extractvalue t st1 cs, sterm_extractvalue t' st1' cs') =>
+  tv_typ t t' && tv_sterm st1 st1' &&
+  sumbool2bool _ _ (list_const_dec cs cs')
+| (sterm_insertvalue t1 st1 t2 st2 cs, 
+   sterm_insertvalue t1' st1' t2' st2' cs') =>
+  tv_typ t1 t1' && tv_sterm st1 st1' && tv_typ t2 t2' && tv_sterm st2 st2' &&
+  sumbool2bool _ _ (list_const_dec cs cs')
+| (sterm_malloc sm t st1 a, sterm_malloc sm' t' st1' a') =>
+  tv_smem sm sm' && tv_typ t t' && tv_sterm st1 st1' && tv_align a a'
+| (sterm_alloca sm t st1 a, sterm_alloca sm' t' st1' a') =>
+  tv_smem sm sm' && tv_typ t t' && tv_sterm st1 st1' && tv_align a a'
+| (sterm_load sm t st1 a, sterm_load sm' t' st1' a') =>
+  tv_smem sm sm' && tv_typ t t' && tv_sterm st1 st1' && tv_align a a'
+| (sterm_gep i t st1 sts2, sterm_gep i' t' st1' sts2') =>
+  sumbool2bool _ _ (bool_dec i i') && tv_typ t t' &&
+  tv_sterm st1 st1' && tv_list_sterm sts2 sts2'
+| (sterm_trunc top t1 st1 t2, sterm_trunc top' t1' st1' t2') =>
+  sumbool2bool _ _ (truncop_dec top top') && tv_typ t1 t1' &&
+  tv_sterm st1 st1' && tv_typ t2 t2'
+| (sterm_ext eo t1 st1 t2, sterm_ext eo' t1' st1' t2') =>
+  sumbool2bool _ _ (extop_dec eo eo') && tv_typ t1 t1' &&
+  tv_sterm st1 st1' && tv_typ t2 t2' 
+| (sterm_cast co t1 st1 t2, sterm_cast co' t1' st1' t2') =>
+  sumbool2bool _ _ (castop_dec co co') && tv_typ t1 t1' &&
+  tv_sterm st1 st1' && tv_typ t2 t2' 
+| (sterm_icmp c t st1 st2, sterm_icmp c' t' st1' st2') =>
+  sumbool2bool _ _ (cond_dec c c') && tv_typ t t' &&
+  tv_sterm st1 st1' && tv_sterm st2 st2'
+| (sterm_fcmp c ft st1 st2, sterm_fcmp c' ft' st1' st2') =>
+  sumbool2bool _ _ (fcond_dec c c') &&
+  sumbool2bool _ _ (floating_point_dec ft ft') &&
+  tv_sterm st1 st1' && tv_sterm st2 st2'
+| (sterm_phi t stls, sterm_phi t' stls') =>
+  tv_typ t t' && tv_list_sterm_l stls stls'
+| (sterm_select st1 t st2 st3, sterm_select st1' t' st2' st3') =>
+  tv_sterm st1 st1' && tv_typ t t' && tv_sterm st2 st2' && tv_sterm st3 st3'
+| (sterm_lib sm i sts, sterm_lib sm' i' sts') =>
+  tv_smem sm sm' && sumbool2bool _ _ (id_dec i i') && tv_list_sterm sts sts'
+| _ => false
+end
+with tv_list_sterm (sts sts':list_sterm) : bool :=
+match (sts, sts') with
+| (Nil_list_sterm, Nil_list_sterm) => true
+| (Cons_list_sterm st sts0, Cons_list_sterm st' sts0') =>
+  tv_sterm st st' && tv_list_sterm sts0 sts0'
+| _ => false
+end
+with tv_list_sterm_l (stls stls':list_sterm_l) : bool :=
+match (stls, stls') with
+| (Nil_list_sterm_l, Nil_list_sterm_l) => true
+| (Cons_list_sterm_l st l stls0, Cons_list_sterm_l st' l' stls0') =>
+  tv_sterm st st' && sumbool2bool _ _ (l_dec l l') && 
+  tv_list_sterm_l stls0 stls0'
+| _ => false
+end
+with tv_smem (sm1 sm2:smem) : bool :=
+match (sm1, sm2) with
+| (smem_init, _) => true
+| (smem_malloc sm1 t1 st1 a1, smem_malloc sm2 t2 st2 a2) =>
+    tv_smem sm1 sm2 && tv_typ t1 t2 && tv_sterm st1 st2 && tv_align a1 a2
+| (smem_alloca sm1 t1 st1 a1, smem_alloca sm2 t2 st2 a2) =>
+    if (tv_typ t1 t2 && tv_sterm st1 st2 && tv_align a1 a2)
+    then tv_smem sm1 sm2
+    else tv_smem (smem_alloca sm1 t1 st1 a1) sm2
+| (smem_free sm1 t1 st1, smem_free sm2 t2 st2) =>
+    tv_smem sm1 sm2 && tv_typ t1 t2 && tv_sterm st1 st2
+| (smem_load sm1 t1 st1 a1, smem_load sm2 t2 st2 a2) =>
+    if (tv_typ t1 t2 && tv_sterm st1 st2 && tv_align a1 a2)
+    then tv_smem sm1 sm2
+    else tv_smem (smem_load sm1 t1 st1 a1) sm2
+| (smem_store sm1 t1 st11 st12 a1, smem_store sm2 t2 st21 st22 a2) =>
+    if (tv_typ t1 t2 && tv_sterm st11 st21 &&
+        tv_sterm st12 st22 && tv_align a1 a2)
+    then tv_smem sm1 sm2
+    else tv_smem (smem_store sm1 t1 st11 st12 a1) sm2
+| (smem_lib sm1 fid1 sts1, smem_lib sm2 fid2 sts2) => 
+    if (sumbool2bool _ _ (id_dec fid1 fid2) && tv_list_sterm sts1 sts2)
+    then tv_smem sm1 sm2
+    else tv_smem (smem_lib sm1 fid1 sts1) sm2
+| (sm1, smem_lib sm2 fid sts) => smem_lib_sub fid && tv_smem sm1 sm2
+| (sm1, smem_alloca sm2 t2 st2 a2) => tv_smem sm1 sm2
+| (sm1, smem_load sm2 t2 st2 a2) => tv_smem sm1 sm2
+| (sm1, smem_store sm2 t2 st21 st22 a2) => tv_smem sm1 sm2
+| _ => false
+end.
+
+Fixpoint tv_sframe (sf1 sf2:sframe) : bool :=
+match (sf1, sf2) with
+| (sframe_init, _) => true
+| (sframe_alloca sm1 sf1 t1 st1 a1, sframe_alloca sm2 sf2 t2 st2 a2) =>
+    if (tv_smem sm1 sm2 && tv_typ t1 t2 && tv_sterm st1 st2 && tv_align a1 a2)
+    then tv_sframe sf1 sf2
+    else tv_sframe (sframe_alloca sm1 sf1 t1 st1 a1) sf2
+| _ => false
+end.
+
+Fixpoint tv_smap (sm1 sm2:smap) : bool :=
+match sm1 with
+| nil => true
+| (id1,st1)::sm1' =>
+  match lookupAL _ sm2 id1 with
+  | None => false
+  | Some st2 => tv_sterm st1 st2 && tv_smap sm1' sm2
+  end
+end.
+Definition sub_sstate s1 s2 := 
+  tv_smap s1.(STerms) s2.(STerms) = true /\ 
+  tv_smem s1.(SMem) s2.(SMem) = true /\
+  tv_sframe s1.(SFrame) s2.(SFrame) = true /\ s1.(SEffects) = s2.(SEffects).
+
+Notation "s1 <<= s2" := (sub_sstate s1 s2) (at level 70, no associativity).
+
+Lemma sstate_sub_dec : forall (sts1 sts2:sstate), 
+  uniq sts1.(STerms) -> {sts1<<=sts2} + {~sts1<<=sts2}.
+Proof.
+Ltac done_right' := 
+  right; intro J ; destruct J as [ J1 [J2 [J3 J4]]]; simpl in *; auto.
+
+  intros sts1 sts2 Huniq.
+  destruct sts1 as [st1 sm1 sf1 se1].
+  destruct sts2 as [st2 sm2 sf2 se2].
+  destruct (@sterms_dec se1 se2); subst; try solve [done_right'].
+  unfold sub_sstate. simpl.
+  destruct (tv_smap st1 st2); auto.
+  destruct (tv_smem sm1 sm2); auto.
+  destruct (tv_sframe sf1 sf2); auto.
+    right. intro J ; destruct J as [ J1 [J2 [J3 J4]]]. inversion J3.
+    right. intro J ; destruct J as [ J1 [J2 [J3 J4]]]. inversion J2.
+    right. intro J ; destruct J as [ J1 [J2 [J3 J4]]]. inversion J1.
+Qed.
 
 Definition tv_cmds (nbs1 nbs2 : list nbranch) :=
 sumbool2bool _ _ (sstate_sub_dec (se_cmds sstate_init nbs1) (se_cmds sstate_init nbs2)
@@ -51,14 +203,23 @@ Axiom tv_fid_injective2 : forall fid1 fid2 fid1' fid2',
  * FunTable. Since the LLVM IR takes function names as function pointers,
  * if a program does not assign them to be other variables, they should
  * be the same. *)
+Fixpoint tv_params (tsts1 tsts2:list (typ*sterm)) : bool :=
+match (tsts1, tsts2) with
+| (nil, _) => true
+| ((t1,st1)::tsts1', (t2,st2)::tsts2') => 
+  tv_typ t1 t2 && tv_sterm st1 st2 && tv_params tsts1' tsts2'
+| _ => false
+end.
+
+(* Do not check if their tailc flags match. Softbound changes the flag for
+ * system calls, say atoi from tailcall to non-tailcall.
+ *)
 Definition tv_scall (c1 c2:scall) :=
-  let '(stmn_call rid1 nr1 tailc1 t1 v1 sts1) := c1 in
-  let '(stmn_call rid2 nr2 tailc2 t2 v2 sts2) := c2 in
+  let '(stmn_call rid1 nr1 _ t1 v1 tsts1) := c1 in
+  let '(stmn_call rid2 nr2 _ t2 v2 tsts2) := c2 in
   (sumbool2bool _ _ (id_dec rid1 rid1)) &&
   (sumbool2bool _ _ (noret_dec nr1 nr2)) &&
-  (sumbool2bool _ _ (tailc_dec tailc1 tailc2)) &&
-  (sumbool2bool _ _ (typ_dec t1 t2)) && 
-  (sumbool2bool _ _ (prefix_dec _ typ_sterm_dec sts1 sts2)) &&
+  tv_typ t1 t2 && tv_params tsts1 tsts2 &&
   match (v1, v2) with
   | (value_const (const_gid _ fid1), value_const (const_gid _ fid2)) => 
       tv_fid fid1 fid2
@@ -84,12 +245,23 @@ match (sbs1, sbs2) with
 | _ => false
 end.
 
-Fixpoint tv_phinodes (ps1 ps2:phinodes) :=
-match (ps1, ps2) with
-| (nil, nil) => true
-| (p1::ps1', p2::ps2') => 
-    sumbool2bool _ _ (phinode_dec p1 p2) && tv_phinodes ps1' ps2'
-| _ => false
+Fixpoint lookupPhinode (phs:phinodes) (i:id) :=
+match phs with
+| nil => None
+| (insn_phi i' t vs)::phs' =>
+    if (eq_dec i i') then Some (insn_phi i' t vs)
+    else lookupPhinode phs' i
+end.
+
+Fixpoint tv_phinodes (ps1 ps2:phinodes) : bool :=
+match ps1 with
+| nil => true
+| (insn_phi i1 _ _)as p1::ps1' =>
+  match lookupPhinode ps2 i1 with
+  | None => false
+  | Some p2 => 
+    sumbool2bool _ _ (phinode_dec p1 p2) && tv_phinodes ps1' ps2
+  end
 end.
 
 Definition tv_block (b1 b2:block) :=
@@ -119,15 +291,15 @@ Definition tv_fheader (f1 f2:fheader) :=
   tv_fid fid1 fid2 &&
   (sumbool2bool _ _ (prefix_dec _ arg_dec a1 a2)).
 
+Definition tv_fdec (f1 f2:fdec) :=
+match (f1, f2) with
+| (fdec_intro fh1, fdec_intro fh2) => tv_fheader fh1 fh2
+end.
+
 Definition tv_fdef (f1 f2:fdef) :=
 match (f1, f2) with
 | (fdef_intro fh1 lb1, fdef_intro fh2 lb2) =>
   tv_fheader fh1 fh2 && tv_blocks lb1 lb2
-end.
-
-Definition tv_fdec (f1 f2:fdec) :=
-match (f1, f2) with
-| (fdec_intro fh1, fdec_intro fh2) => tv_fheader fh1 fh2
 end.
 
 Fixpoint lookupGvarViaIDFromProducts (lp:products) (i:id) : option gvar :=
@@ -139,272 +311,40 @@ match lp with
 | _::lp' => lookupGvarViaIDFromProducts lp' i
 end.
 
-Definition products_sub (Ps1 Ps2:products) := forall id1, 
-  In id1 (getProductsIDs Ps1) ->
-  (forall fdec1,
-    lookupFdecViaIDFromProducts Ps1 id1 = Some fdec1 ->
-    exists fdec2,
-      lookupFdecViaIDFromProducts Ps2 (rename_fid id1) = Some fdec2 /\ 
-      tv_fdec fdec1 fdec2 = true)
-  /\
-  (forall fdef1,
-    lookupFdefViaIDFromProducts Ps1 id1 = Some fdef1 ->
-    exists fdef2,
-      lookupFdefViaIDFromProducts Ps2 (rename_fid id1) = Some fdef2 /\ 
-      tv_fdef fdef1 fdef2 = true)
-  /\
-  (forall gv1,
-    lookupGvarViaIDFromProducts Ps1 id1 = Some gv1 ->
-    exists gv2,
-      lookupGvarViaIDFromProducts Ps2 id1 = Some gv2 /\ 
-      sumbool2bool _ _ (gvar_dec gv1 gv2) = true).
+Fixpoint tv_products (Ps1 Ps2:products) : bool :=
+match Ps1 with
+| nil => true
+| product_gvar gv1::Ps1' =>
+  match lookupGvarViaIDFromProducts Ps2 (getGvarID gv1) with
+  | None => false
+  | Some gv2 => sumbool2bool _ _ (gvar_dec gv1 gv2) && tv_products Ps1' Ps2 
+  end
+| product_fdec f1::Ps1' =>
+  match lookupFdecViaIDFromProducts Ps2 (rename_fid (getFdecID f1)) with
+  | None => false
+  | Some f2 => tv_fdec f1 f2 && tv_products Ps1' Ps2 
+  end
+| product_fdef f1::Ps1' =>
+  match lookupFdefViaIDFromProducts Ps2 (rename_fid (getFdefID f1)) with
+  | None => false
+  | Some f2 => tv_fdef f1 f2 && tv_products Ps1' Ps2 
+  end
+end.
 
-(*
-Lemma lookupAL_app1 : forall X (lc1:list (atom*X)) lc2 i,
-  i `in` dom lc1 ->
-  lookupAL X lc1 i = lookupAL X (lc1++lc2) i.
-Proof.
-  induction lc1; intros lc2 i Hi_in_lc1.
-    fsetdec.
-    destruct a as (id, elt); simpl in *.
-    destruct (@eq_dec atom (EqDec_eq_of_EqDec atom EqDec_atom) i id); auto.
-      apply IHlc1. fsetdec.
-Qed.    
+Definition tv_module (m1 m2:module) :=
+match (m1, m2) with
+| (module_intro los1 nts1 Ps1, module_intro los2 nts2 Ps2) =>
+  sumbool2bool _ _ (layouts_dec los1 los2) &&
+  sumbool2bool _ _ (namedts_dec nts1 nts2) &&
+  tv_products Ps1 Ps2
+end.
 
-Lemma lookupAL_app2 : forall X lc1 (lc2:list (atom*X)) i,
-  i `notin` dom lc1 ->
-  lookupAL X lc2 i = lookupAL X (lc1++lc2) i.
-Proof.
-  induction lc1; intros lc2 i Hi_notin_lc1; auto.
-    destruct a as (id, elt); simpl in *.
-    destruct (@eq_dec atom (EqDec_eq_of_EqDec atom EqDec_atom) i id); subst; eauto.
-      fsetdec.
-Qed.    
-*)
-
-Lemma products_sub_app1 : forall Ps1 Ps2 Ps,
-  products_sub Ps1 Ps -> 
-  products_sub Ps2 Ps ->
-  products_sub (Ps1++Ps2) Ps.
-Proof.
-  intros Ps1 Ps2 Ps HPs1_sub_Ps HPs2_sub_Ps.
-  intros i i_in_Ps12.
-(*
-  simpl_env in i_in_lc12.
-  apply in_dom_app_inv in i_in_lc12.
-  assert (i `in`  dom lc1 \/ i `notin` dom lc1) as i_in_lc1_dec. fsetdec.
-  destruct i_in_lc1_dec as [i_in_lc1 | i_notin_lc1].
-    rewrite <- Hlc1_sub_lc; auto.
-    rewrite <- lookupAL_app1; auto.
-
-    destruct i_in_lc12 as [i_in_lc1 | i_in_lc2].
-      fsetdec.
-      rewrite <- lookupAL_app2; auto.
-*)
-Admitted.
-
-(*
-Lemma lookupALs_tail : forall X l2b l2b' l0,
-  l0 `notin` dom l2b ->
-  lookupAL X (l2b++l2b') l0 = lookupAL _ l2b' l0.
-Proof.
-  intros.
-  induction l2b; auto.
-    destruct a. simpl in *.
-    destruct (@eq_dec atom (@EqDec_eq_of_EqDec atom EqDec_atom) l0 a); subst; auto.
-      fsetdec.
-Qed.
-*)
-
-Lemma products_sub_app2 : forall Ps1 Ps2 Ps,
-  products_sub Ps1 Ps -> 
-  NoDup (getProductsIDs (Ps1++Ps2)) ->
-  ~ products_sub Ps2 Ps ->
-  ~ products_sub (Ps1++Ps2) Ps.
-Admitted.
-(*
-Proof.
-  intros X lc1 lc2 lc Hlc1_sub_lc Hdisj Hlc2_nsub_lc Hlc12_sub_lc.
-  apply Hlc2_nsub_lc.
-  intros i i_in_lc2.
-    assert (i `notin` dom lc1) as i_notin_lc1. solve_uniq.
-    assert (i `in` dom (lc1++lc2)) as i_in_lc12. simpl_env. fsetdec.
-    apply Hlc12_sub_lc in i_in_lc12.
-    erewrite lookupALs_tail in i_in_lc12; eauto.
-Qed.
-*)
-
-Lemma products_sub_dec: forall Ps1 Ps2, 
-  NoDup (getProductsIDs Ps1) ->
-  {products_sub Ps1 Ps2} + {~products_sub Ps1 Ps2}.
-Proof.
-  induction Ps1; intros Ps2 Huniq.
-    left. intros id1 Hindom. 
-    inversion Hindom.
-
-    simpl in Huniq.
-    rewrite_env (nil ++ getProductID a :: getProductsIDs Ps1) in Huniq.
-    assert (Hnotindom:=Huniq).
-    apply NoDup_remove_2 in Hnotindom.
-    assert (Huniq':=Huniq).
-    apply NoDup_remove_1 in Huniq'.
-    simpl_env in *.
-    destruct a as [g1 | f1 | f1].
-    Case "gvar".
-      remember (lookupGvarViaIDFromProducts Ps2 (getGvarID g1)) as Lookup.
-      destruct Lookup as [g2 | ].
-      SCase "gid in Ps2".
-        destruct (gvar_dec g1 g2); subst.
-        SSCase "g1 = g2".
-          assert (products_sub [product_gvar g2] Ps2) as Hg2_sub_Ps2.
-            intros i Hi_in_dom. simpl. 
-            repeat split; try solve [intros a Hlookup; inversion Hlookup].
-            intros gv1 Hlookup.
-            destruct (@eq_dec id (EqDec_eq_of_EqDec id EqDec_atom) (getGvarID g2) i); inversion Hlookup; subst.
-              exists gv1. split; auto.
-              destruct (gvar_dec gv1 gv1); simpl; auto.
-          destruct (@IHPs1 Ps2 Huniq') as [HPs1_sub_Ps2 | HPs1_nsub_Ps2].
-            left. apply products_sub_app1; auto.
-            right. apply products_sub_app2; auto.
-          
-        SSCase "g1 <> g2".
-          right. intro J.
-          assert (In (getGvarID g1) (getProductsIDs ([product_gvar g1]++Ps1))) 
-            as Hindom. 
-            simpl. auto.
-          assert (H:=@J (getGvarID g1) Hindom). simpl in H.
-          destruct H as [_ [_ H3]].
-          destruct (@eq_dec id (EqDec_eq_of_EqDec id EqDec_atom) (getGvarID g1) (getGvarID g1)) as [e | n']; try solve [contradict n'; auto].
-          destruct (@H3 g1) as [gv2 [J1 J2]]; auto.
-          rewrite <- HeqLookup in J1. inversion J1; subst.
-          destruct (gvar_dec g1 gv2); subst; auto.
-            simpl in J2. inversion J2.
-
-      SCase "gid notin Ps2".
-        right. intro J.
-        assert (In (getGvarID g1) (getProductsIDs ([product_gvar g1]++Ps1))) 
-          as Hindom. 
-          simpl. auto.
-        assert (H:=@J (getGvarID g1) Hindom). simpl in H.
-        destruct H as [H1 [H2 H3]].
-        destruct (@eq_dec id (EqDec_eq_of_EqDec id EqDec_atom) (getGvarID g1) (getGvarID g1)) as [e | n']; try solve [contradict n'; auto].
-        destruct (@H3 g1) as [gv2 [J1 J2]]; auto.       
-        rewrite <- HeqLookup in J1. inversion J1.
-        
-    Case "fdec".
-      remember (lookupFdecViaIDFromProducts Ps2 (rename_fid (getFdecID f1))) as Lookup.
-      destruct Lookup as [f2 | ].
-      SCase "fid in Ps2".
-        remember (tv_fdec f1 f2) as R.
-        destruct R; subst.
-        SSCase "f1 = f2".
-          assert (products_sub [product_fdec f1] Ps2) as Hf2_sub_Ps2.
-            intros i Hi_in_dom. simpl. 
-            repeat split; try solve [intros a Hlookup; inversion Hlookup].
-            intros fdec1 Hlookup.
-            destruct (@eq_dec id (EqDec_eq_of_EqDec id EqDec_atom) (getFdecID f1) i); inversion Hlookup; subst.
-              exists f2. split; auto.
-          destruct (@IHPs1 Ps2 Huniq') as [HPs1_sub_Ps2 | HPs1_nsub_Ps2].
-            left. apply products_sub_app1; auto.
-            right. apply products_sub_app2; auto.
-          
-        SSCase "f1 <> f2".
-          right. intro J.
-          assert (In (getFdecID f1) (getProductsIDs ([product_fdec f1]++Ps1))) 
-            as Hindom. 
-            simpl. auto.
-          assert (H:=@J (getFdecID f1) Hindom). simpl in H.
-          destruct H as [H1 _].
-          destruct (@eq_dec id (EqDec_eq_of_EqDec id EqDec_atom) (getFdecID f1) (getFdecID f1)) as [e | n']; try solve [contradict n'; auto].
-          destruct (@H1 f1) as [fdec2 [J1 J2]]; auto.
-          rewrite <- HeqLookup in J1. inversion J1; subst.
-          rewrite J2 in HeqR. inversion HeqR.
-
-      SCase "fid notin Ps2".
-        right. intro J.
-        assert (In (getFdecID f1) (getProductsIDs ([product_fdec f1]++Ps1))) 
-          as Hindom. 
-          simpl. auto.
-        assert (H:=@J (getFdecID f1) Hindom). simpl in H.
-        destruct H as [H1 [H2 H3]].
-        destruct (@eq_dec id (EqDec_eq_of_EqDec id EqDec_atom) (getFdecID f1) (getFdecID f1)) as [e | n']; try solve [contradict n'; auto].
-        destruct (@H1 f1) as [fdec2 [J1 J2]]; auto.       
-        rewrite <- HeqLookup in J1. inversion J1.
-
-    Case "fdef".
-      remember (lookupFdefViaIDFromProducts Ps2 (rename_fid (getFdefID f1))) as Lookup.
-      destruct Lookup as [f2 | ].
-      SCase "fid in Ps2".
-        remember (tv_fdef f1 f2) as R.
-        destruct R; subst.
-        SSCase "f1 = f2".
-          assert (products_sub [product_fdef f1] Ps2) as Hf2_sub_Ps2.
-            intros i Hi_in_dom. simpl. 
-            repeat split; try solve [intros a Hlookup; inversion Hlookup].
-            intros fdef1 Hlookup.
-            destruct (@eq_dec id (EqDec_eq_of_EqDec id EqDec_atom) (getFdefID f1) i); inversion Hlookup; subst.
-              exists f2. split; auto.
-          destruct (@IHPs1 Ps2 Huniq') as [HPs1_sub_Ps2 | HPs1_nsub_Ps2].
-            left. apply products_sub_app1; auto.
-            right. apply products_sub_app2; auto.
-          
-        SSCase "f1 <> f2".
-          right. intro J.
-          assert (In (getFdefID f1) (getProductsIDs ([product_fdef f1]++Ps1))) 
-            as Hindom. 
-            simpl. auto.
-          assert (H:=@J (getFdefID f1) Hindom). simpl in H.
-          destruct H as [_ [H2 _]].
-          destruct (@eq_dec id (EqDec_eq_of_EqDec id EqDec_atom) (getFdefID f1) (getFdefID f1)) as [e | n']; try solve [contradict n'; auto].
-          destruct (@H2 f1) as [fdef2 [J1 J2]]; auto.
-          rewrite <- HeqLookup in J1. inversion J1; subst.
-          rewrite J2 in HeqR. inversion HeqR.
-
-      SCase "fid notin Ps2".
-        right. intro J.
-        assert (In (getFdefID f1) (getProductsIDs ([product_fdef f1]++Ps1))) 
-          as Hindom. 
-          simpl. auto.
-        assert (H:=@J (getFdefID f1) Hindom). simpl in H.
-        destruct H as [_ [H2 _]].
-        destruct (@eq_dec id (EqDec_eq_of_EqDec id EqDec_atom) (getFdefID f1) (getFdefID f1)) as [e | n']; try solve [contradict n'; auto].
-        destruct (@H2 f1) as [fdec2 [J1 J2]]; auto.       
-        rewrite <- HeqLookup in J1. inversion J1.
-Qed.
-
-Lemma tv_products: forall (Ps1 Ps2:products), NoDup (getProductsIDs Ps1) -> bool.
-Proof.
-  intros Ps1 Ps2 Huniq.
-  apply (sumbool2bool _ _ (products_sub_dec Ps1 Ps2 Huniq)).
-Defined.
-
-Lemma tv_module : forall (m1 m2:module), uniqModule m1 -> bool.
-Proof.
-  intros m1 m2 Huniq.
-  destruct m1 as [los1 nts1 Ps1].
-  destruct m2 as [los2 nts2 Ps2].
-  destruct Huniq as [_ [_ Huniq]].
-  apply (sumbool2bool _ _ (layouts_dec los1 los2) &&
-         sumbool2bool _ _ (namedts_dec nts1 nts2) &&
-         tv_products Ps1 Ps2 Huniq).
-Defined.
-
-Lemma tv_system : forall (S1 S2:system), uniqSystem S1 -> bool.
-Proof.
-  induction S1 as [ | m1 S1]; intros S2 Huniq.
-    destruct S2.
-      apply true.
-      apply false.
-
-    destruct S2 as [ | m2 S2].
-      apply false.
-
-      assert (uniqModule m1) as Huniq1.
-        inversion Huniq; auto.
-      assert (uniqSystem S1) as Huniq2.
-        inversion Huniq; auto.
-      apply (tv_module m1 m2 Huniq1 && IHS1 S2 Huniq2).
-Defined.
+Fixpoint tv_system (S1 S2:system) :=
+match (S1, S2) with
+| (nil, nil) => true
+| (m1::S1', m2::S2') => tv_module m1 m2 && tv_system S1' S2'
+| _ => false
+end.
 
 Ltac sumbool_simpl :=
   repeat
